$$
\begin{bmatrix}
y_0\\y_1\\y_2\\y_3\\.\\.\\y_{n-1}
\end{bmatrix}
=
\begin{bmatrix}
1&1&1&1&...&1\\
1&\omega_n&\omega_n^2&\omega_n^3&...&\omega_n^{n-1}\\
1&\omega_n^2&\omega_n^4&\omega_n^6&...&\omega_n^{2(n-1)}\\
1&\omega_n^3&\omega_n^6&\omega_n^9&...&\omega_n^{3(n-1)}\\
...&...&...&...&...&...\\
1&\omega_n^{n-1}&\omega_n^{2(n-1)}&\omega_n^{3(n-1)}&...&\omega_n^{(n-1)(n-1)}
\end{bmatrix}
*
\begin{bmatrix}
a_0\\a_1\\a_2\\a_3\\.\\.\\a_{n-1}
\end{bmatrix}
$$

$$
[V_n^{-1}V_n]_{jj'}=\sum\limits_{k=0}^{n-1}(\omega_n^{-kj}/n)(\omega_n^{kj'})=\sum\limits_{k=0}^{n-1}\omega_n^{k(j'-j)}/n
$$

，具体证明如下，摘自算导：

　　　　　$[V_n^{-1}V_n]_{jj'}=\sum\limits_{k=0}^{n-1}(\omega_n^{-kj}/n)(\omega_n^{kj'})=\sum\limits_{k=0}^{n-1}\omega_n^{k(j'-j)}/n$

　　　　　若$j=j'$，则结果为1；否则根据求和引理，结果为0。那么这个乘积就是单位矩阵，得证$V_n^{-1}$为$V_n$的逆矩阵。